Implement rest of optimization

extraction/theories/Optimize.v
@@ -1,5 +1,4 @@
 From ConCert.Extraction Require Import Erasure.
-From ConCert.Extraction Require Import ESubterm.
 From ConCert.Extraction Require Import ExAst.
 From ConCert.Extraction Require Import ExTyping.
 From ConCert.Extraction Require Import StringExtra.
@@ -9,6 +8,7 @@ From Coq Require Import Ascii.
 From Coq Require Import Bool.
 From Coq Require Import List.
 From Coq Require Import PArith.
+From Coq Require Import Psatz.
 From Coq Require Import String.
 From Coq Require VectorDef.
 From Equations Require Import Equations.
@@ -38,32 +38,6 @@ Definition inspect {A} (x : A) : { a | a = x } :=
 
 (* Eta expand all constructors so they are applied to all their parameters *)
 Section eta.
-Context (Σ : global_env).
-
-Definition mcΣ : EAst.global_declarations :=
-  map (fun '(kn, cst) =>
-         (kn,
-          match cst with
-          | ConstantDecl cst =>
-            EAst.ConstantDecl {| EAst.cst_body := cst_body cst |}
-          | InductiveDecl mib =>
-            EAst.InductiveDecl
-              {| EAst.ind_npars := ind_npars mib;
-                 EAst.ind_bodies :=
-                   map (fun oib =>
-                          {| EAst.ind_name := ind_name oib;
-                             EAst.ind_kelim := InType;
-                             EAst.ind_ctors :=
-                               map (fun '(name, data) => (name, tBox, List.length data))
-                                   (ind_ctors oib);
-                             EAst.ind_projs :=
-                               map (fun '(name, bt) => (name, tBox))
-                                   (ind_projs oib) |})
-                       (ind_bodies mib) |}
-          end))
-      Σ.
-
-Section eta.
 (* Ctors to eta expand *)
 Context (ctors : list (inductive * nat * nat)).
 (* Constants to eta expand *)
@@ -91,6 +65,20 @@ Definition eta_const (kn : kername) (args : list term) : term :=
   | None => mkApps (tConst kn) args
   end.
 
+(*
+Fixpoint decompose_lam_upto_n (n : nat) (t : term) : list name * term :=
+  match n, t with
+  | S n, tLambda na t => let (nas, t) := decompose_lam_upto_n n t in
+                         (na :: nas, t)
+  | _, _ => ([], t)
+  end.
+
+(* Unfortunate MetaCoq's typing does not impose any conditions on the shape of
+   case branches, so we also have to eta expand those... *)
+Definition eta_cases (ind : inductive) (brs : list (nat * term)) : list (nat * term) :=
+  brs. (* todo *)
+*)
+
 Definition map_subterms (f : term -> term) (t : term) : term :=
   match t with
   | tEvar n ts => tEvar n (map f ts)
@@ -105,15 +93,37 @@ Definition map_subterms (f : term -> term) (t : term) : term :=
   | t => t
   end.
 
-Fixpoint eta_expand (args : list term) (t : term) : term :=
+Fixpoint eta_expand_aux (args : list term) (t : term) : term :=
   match t with
-  | tApp hd arg => eta_expand (eta_expand [] arg :: args) hd
+  | tApp hd arg => eta_expand_aux (eta_expand_aux [] arg :: args) hd
   | tConstruct ind c => eta_ctor ind c args
   | tConst kn => eta_const kn args
-  | t => mkApps (map_subterms (eta_expand []) t) args
+  (*| tCase (ind, npars) disc brs =>
+    mkApps
+      (tCase
+         (ind, npars)
+         (eta_expand_aux [] disc)
+         (eta_cases ind (map (on_snd (eta_expand_aux [])) brs)))
+      args*)
+  | t => mkApps (map_subterms (eta_expand_aux []) t) args
   end.
 
-Lemma wfe_term_eta_single t args n :
+Definition eta_expand (t : term) : term :=
+  eta_expand_aux [] t.
+
+Definition eta_expand_decl (decl : global_decl) : global_decl :=
+  match decl with
+  | ConstantDecl cst =>
+    ConstantDecl
+      {| cst_type := cst_type cst;
+         cst_body := option_map eta_expand (cst_body cst) |}
+  | _ => decl
+  end.
+
+Definition eta_expand_env (Σ : global_env) : global_env :=
+  map (on_snd eta_expand_decl) Σ.
+
+Lemma wfe_term_eta_single Σ t args n :
   wfe_term Σ t ->
   Forall (wfe_term Σ) args ->
   wfe_term Σ (eta_single t args n).
@@ -136,7 +146,7 @@ Proof.
     constructor; easy.
 Qed.
 
-Lemma wfe_term_eta_ctor ind i args :
+Lemma wfe_term_eta_ctor Σ ind i args :
   wfe_term Σ (tConstruct ind i) ->
   Forall (wfe_term Σ) args ->
   wfe_term Σ (eta_ctor ind i args).
@@ -148,7 +158,7 @@ Proof.
   - now apply wfe_term_mkApps.
 Qed.
 
-Lemma wfe_term_eta_const kn args :
+Lemma wfe_term_eta_const Σ kn args :
   wfe_term Σ (tConst kn) ->
   Forall (wfe_term Σ) args ->
   wfe_term Σ (eta_const kn args).
@@ -160,10 +170,10 @@ Proof.
   - now apply wfe_term_mkApps.
 Qed.
 
-Lemma wfe_term_eta_expand args t :
+Lemma wfe_term_eta_expand_aux Σ args t :
   Forall (wfe_term Σ) args ->
   wfe_term Σ t ->
-  wfe_term Σ (eta_expand args t).
+  wfe_term Σ (eta_expand_aux args t).
 Proof.
   revert args.
   induction t using term_forall_list_ind; intros args wfall wft; cbn in *; auto.
@@ -193,6 +203,11 @@ Proof.
     induction H; cbn in *; easy.
 Qed.
 
+Lemma wfe_term_eta_expand Σ t :
+  wfe_term Σ t ->
+  wfe_term Σ (eta_expand t).
+Proof. now apply wfe_term_eta_expand_aux. Qed.
+
 Lemma decompose_app_rec_app t acc acc' :
   let (hd, args) := decompose_app_rec t acc in
   decompose_app_rec t (acc ++ acc') = (hd, args ++ acc').
@@ -204,12 +219,14 @@ Proof.
   now rewrite <- app_comm_cons in IHt1.
 Qed.
 
-Lemma eta_expand_unfold t args :
-  eta_expand args t =
+Lemma eta_expand_aux_unfold t args :
+  eta_expand_aux args t =
   match decompose_app t with
-  | (tConstruct ind c, args') => eta_ctor ind c (map (eta_expand []) args' ++ args)
-  | (tConst kn, args') => eta_const kn (map (eta_expand []) args' ++ args)
-  | (hd, args') => mkApps (map_subterms (eta_expand []) hd) (map (eta_expand []) args' ++ args)
+  | (tConstruct ind c, args') => eta_ctor ind c (map (eta_expand_aux []) args' ++ args)
+  | (tConst kn, args') => eta_const kn (map (eta_expand_aux []) args' ++ args)
+  | (hd, args') => mkApps
+                     (map_subterms (eta_expand_aux []) hd)
+                     (map (eta_expand_aux []) args' ++ args)
   end.
 Proof.
   revert args.
@@ -226,36 +243,265 @@ Proof.
   now rewrite <- app_assoc.
 Qed.
 
-Lemma eta_expand_nil_unfold t :
-  eta_expand [] t =
+Lemma eta_expand_unfold t :
+  eta_expand t =
   match decompose_app t with
-  | (tConstruct ind c, args) => eta_ctor ind c (map (eta_expand []) args)
-  | (tConst kn, args) => eta_const kn (map (eta_expand []) args)
-  | (hd, args) => mkApps (map_subterms (eta_expand []) hd) (map (eta_expand []) args)
+  | (tConstruct ind c, args) => eta_ctor ind c (map eta_expand args)
+  | (tConst kn, args) => eta_const kn (map eta_expand args)
+  | (hd, args) => mkApps (map_subterms eta_expand hd) (map eta_expand args)
   end.
 Proof.
-  rewrite eta_expand_unfold.
+  unfold eta_expand at 1.
+  rewrite eta_expand_aux_unfold.
   destruct (decompose_app _).
   now rewrite app_nil_r.
 Qed.
 
-Notation "s ▷ t" := (eval mcΣ s t) (at level 50, t at next level) : type_scope.
 
 End eta.
 
+Local Open Scope positive.
 Definition set_bit (n : nat) (p : positive) : positive :=
   Pos.lor p (Pos.shiftl_nat 1 n).
 
 Definition has_bit (n : nat) (p : positive) : bool :=
   Pos.testbit_nat p n.
 
-Local Open Scope positive.
 Definition chop (p : positive) : positive :=
   match p with
   | p~0 => p
   | p~1 => p
   | XH => 1
   end.
+
+Fixpoint bitmask_zeros (n : nat) : positive :=
+  match n with
+  | 0%nat => xH
+  | S n => (bitmask_zeros n)~0
+  end.
+
+Fixpoint bitmask_ones (n : nat) : positive :=
+  match n with
+  | 0%nat => xH
+  | S n => (bitmask_ones n)~1
+  end.
+
+Fixpoint lnot (p : positive) : positive :=
+  match p with
+  | p~0 => (lnot p)~1
+  | p~1 => (lnot p)~0
+  | xH => xH
+  end.
+
+(* Returns successor of the index of the last 1 in the bitmask *)
+Definition S_last_1 (p : positive) : nat :=
+  (fix f p i n :=
+     match p with
+     | xH => n
+     | p~0 => f p (S i) n
+     | p~1 => f p (S i) (S i)
+     end) p 0%nat 0%nat.
+
+Local Open Scope nat.
+Fixpoint skip_mask (n : nat) (p : positive) : positive :=
+  match n with
+  | 0 => p
+  | S n => skip_mask n (chop p)
+  end.
+
+Section dearg.
+(* We are given bitmasks representing which args to remove *)
+Context (ctors : list (inductive * nat * positive)).
+Context (constants : list (kername * positive)).
+
+Fixpoint unlift (n k : nat) (t : term) : term :=
+  match t with
+  | tRel i => if k <=? i then tRel (i - n) else tRel i
+  | tEvar ev args => tEvar ev (map (unlift n k) args)
+  | tLambda na M => tLambda na (unlift n (S k) M)
+  | tLetIn na b b' => tLetIn na (unlift n k b) (unlift n (S k) b')
+  | tApp u v => tApp (unlift n k u) (unlift n k v)
+  | tCase ind c brs => let brs' := map (on_snd (unlift n k)) brs in tCase ind (unlift n k c) brs'
+  | tProj p c => tProj p (unlift n k c)
+  | tFix mfix idx =>
+    let k' := #|mfix| + k in
+    let mfix' := map (map_def (unlift n k')) mfix in
+    tFix mfix' idx
+  | tCoFix mfix idx =>
+    let k' := #|mfix| + k in
+    let mfix' := map (map_def (unlift n k')) mfix
+    in tCoFix mfix' idx
+  | _ => t
+  end.
+
+Fixpoint dearg_single (mask : positive) (t : term) (args : list term) : term :=
+  match mask, args with
+  | mask~1, arg :: args => dearg_single mask t args
+  | mask~0, arg :: args => dearg_single mask (tApp t arg) args
+  | _, _ => mkApps t args
+            (* todo: pass through conditions saying that we never run out of args, only mask? *)
+  end.
+
+Definition dearg_ctor (ind : inductive) (c : nat) (args : list term) : term :=
+  match find (fun '(ind', c', _) => eq_inductive ind' ind && (c' =? c)) ctors with
+  | Some (_, _, mask) => dearg_single mask (tConstruct ind c) args
+  | None => mkApps (tConstruct ind c) args
+  end.
+
+Definition dearg_const (kn : kername) (args : list term) : term :=
+  match find (fun '(kn', _) => eq_kername kn' kn) constants with
+  | Some (_, mask) => dearg_single mask (tConst kn) args
+  | None => mkApps (tConst kn) args
+  end.
+
+Fixpoint dearg_lambdas (mask : positive) (ar : nat) (t : term) : nat * term :=
+  match mask, t with
+  | mask~1, tLambda na body => dearg_lambdas mask (ar - 1) (unlift 1 0 body)
+  | mask~0, tLambda na body => let (ar, t) := dearg_lambdas mask ar body in
+                               (ar, tLambda na t)
+  | _, _ => (ar, t)
+  end.
+
+Definition dearg_case_branches
+           (ind : inductive)
+           (npars : nat)
+           (brs : list (nat * term)) : list (nat * term) :=
+  let dearg_one c br :=
+      match find (fun '(ind', c', _) => eq_inductive ind' ind && (c' =? c)) ctors with
+      | Some (_, _, mask) => dearg_lambdas (skip_mask npars mask) br.1 br.2
+      | None => br
+      end in
+  mapi dearg_one brs.
+
+Fixpoint dearg_aux (args : list term) (t : term) : term :=
+  match t with
+  | tApp hd arg => dearg_aux (dearg_aux [] arg :: args) hd
+  | tConstruct ind c => dearg_ctor ind c args
+  | tConst kn => dearg_const kn args
+  | tCase (ind, npars) discr brs =>
+    (* todo: what to do about parameters? Right now we remove them
+       in a separate pass. *)
+    mkApps
+      (tCase
+         (ind, npars)
+         (dearg_aux [] discr)
+         (dearg_case_branches ind npars (map (on_snd (dearg_aux [])) brs)))
+      args
+  | t => mkApps (map_subterms (dearg_aux []) t) args
+  end.
+
+(* Remove lambda abstractions from top level declaration based on bitmask *)
+Fixpoint dearg_cst_top
+         (mask : positive)
+         (type : box_type)
+         (body : term) : box_type * term :=
+  match mask, type, body with
+  | _, _, tLetIn na val body =>
+    let (type, body) := dearg_cst_top mask type body in
+    (type, tLetIn na val body)
+  | mask~1, TArr _ cod, tLambda _ body =>
+    let (type, body) := dearg_cst_top mask cod body in
+    (type, unlift 1 0 body)
+  | mask~0, TArr dom cod, tLambda na body =>
+    let (cod, body) := dearg_cst_top mask cod body in
+    (TArr dom cod, tLambda na body)
+  | _, _, _ => (type, body)
+  end.
+
+(* Remove lambda abstractions from top level declaration and remove
+   all unused args in applicacations *)
+Definition dearg_cst (kn : kername) (cst : constant_body) : constant_body :=
+  let cst :=
+      match find (fun '(kn', _) => eq_kername kn' kn) constants with
+      | Some (_, _, mask) =>
+        match cst_body cst with
+        | Some body =>
+          let (new_type, new_body) := dearg_cst_top mask (cst_type cst).2 body in
+          {| cst_type := ((cst_type cst).1, new_type); cst_body := Some new_body |}
+        | None => cst
+        end
+      | None => cst
+      end in
+  {| cst_type := cst_type cst; cst_body := option_map (dearg_aux []) (cst_body cst) |}.
+
+(* Remove all data from ctor based on bitmask *)
+Fixpoint dearg_oib_ctor (mask : positive) (bts : list box_type) : list box_type :=
+  match mask, bts with
+  | mask~0, bt :: bts => bt :: dearg_oib_ctor mask bts
+  | mask~1, bt :: bts => dearg_oib_ctor mask bts
+  | _, _ => bts
+  end.
+
+Definition dearg_oib (ind : inductive) (oib : one_inductive_body) : one_inductive_body :=
+  {| ind_name := ind_name oib;
+     ind_type_vars := ind_type_vars oib;
+     ind_ctors :=
+       mapi (fun c '(name, bts) =>
+               match find (fun '(ind', c', _) => eq_inductive ind' ind && (c' =? c)) ctors with
+               | Some (_, _, mask) => (name, dearg_oib_ctor mask bts)
+               | None => (name, bts)
+               end)
+            (ind_ctors oib);
+     ind_projs := ind_projs oib |}.
+
+Definition dearg_mib (kn : kername) (mib : mutual_inductive_body) : mutual_inductive_body :=
+  {| ind_npars := ind_npars mib;
+     ind_bodies := mapi (fun i => dearg_oib {| inductive_mind := kn;
+                                               inductive_ind := i |})
+                        (ind_bodies mib) |}.
+
+Definition dearg_decl (kn : kername) (decl : global_decl) : global_decl :=
+  match decl with
+  | ConstantDecl cst => ConstantDecl (dearg_cst kn cst)
+  | InductiveDecl mib => InductiveDecl (dearg_mib kn mib)
+  end.
+
+Definition dearg_env (Σ : global_env) : global_env :=
+  map (fun '(kn, decl) => (kn, dearg_decl kn decl)) Σ.
+
+End dearg.
+
+Local Open Scope nat.
+Fixpoint delete_parameters_term (t : term) : term :=
+  match t with
+  | tCase (ind, npars) discr brs =>
+    tCase (ind, 0) (delete_parameters_term discr) (map (on_snd delete_parameters_term) brs)
+  | t => map_subterms delete_parameters_term t
+  end.
+
+Definition delete_parameters_decl (decl : global_decl) : global_decl :=
+  match decl with
+  | ConstantDecl cst =>
+    ConstantDecl
+      {| cst_type := cst_type cst;
+         cst_body := option_map delete_parameters_term (cst_body cst); |}
+  | InductiveDecl mib =>
+    InductiveDecl
+      {| ind_npars := 0;
+         ind_bodies := ind_bodies mib |}
+  end.
+
+Definition make_parameter_dearg_masks (Σ : global_env) : list (inductive * nat * positive) :=
+  flat_map
+    (fun '(kn, decl) =>
+       match decl with
+       | InductiveDecl mib =>
+         let mask := bitmask_ones (ind_npars mib) in
+         let oib_ctors i oib :=
+             let ind := {| inductive_mind := kn; inductive_ind := i |} in
+             mapi (fun c _ => (ind, c, mask)) (ind_ctors oib) in
+         List.concat (mapi oib_ctors (ind_bodies mib))
+       | _ => []
+       end)
+    Σ.
+
+(* Remove parameters from all inductives *)
+Definition remove_parameters (Σ : global_env) : global_env :=
+  let ctors := make_parameter_dearg_masks Σ in
+  let ctors_eta_count := map (fun '(ind, c, mask) => (ind, c, S_last_1 mask)) ctors in
+  let Σ := eta_expand_env ctors_eta_count [] Σ in
+  let Σ := dearg_env ctors [] Σ in
+  map (on_snd delete_parameters_decl) Σ.
 
 (* Return bitmask indicating which context variables have uses *)
 Fixpoint used_context_vars (Γ : positive) (t : term) : positive :=
@@ -277,6 +523,82 @@ Fixpoint used_context_vars (Γ : positive) (t : term) : positive :=
   | tCoFix def _ => fold_right Pos.lor Γ (map (used_context_vars Γ ∘ dbody) def)
   end.
 
+(* Return bitmask indicating which parameters are used by the
+specified lambda abstractions. All parameters after the end of
+the bit mask should be assumed to be used. *)
+Fixpoint func_body_used_params (Γ : positive) (t : term) (ty : box_type) : positive :=
+  match t, ty with
+  | tLetIn na val body, ty =>
+    let Γ := used_context_vars Γ val in
+    chop (func_body_used_params Γ~0 body ty)
+  | tLambda na body, TArr hd ty =>
+    func_body_used_params Γ~0 body ty
+  | t, ty => used_context_vars Γ t
+  end.
+
+Fixpoint bitmask_rev_aux (p : positive) (acc : positive) : positive :=
+  match p with
+  | xH => acc
+  | p~0 => bitmask_rev_aux p (acc~0)
+  | p~1 => bitmask_rev_aux p (acc~1)
+  end.
+
+Definition bitmask_rev (p : positive) : positive :=
+  bitmask_rev_aux p xH.
+
+Definition constant_used_params (cst : constant_body) : positive :=
+  match cst_body cst with
+  | None => xH
+  | Some body => bitmask_rev (func_body_used_params xH body (cst_type cst).2)
+  end.
+
+Fixpoint mask_from_ctor_types (bts : list box_type) : positive :=
+  match bts with
+  | [] => xH
+  | TBox :: bts
+  | TAny :: bts => (mask_from_ctor_types bts)~0
+  | _ :: bts => (mask_from_ctor_types bts)~1
+  end.
+
+Definition ind_ctors_used_params
+           (kn : kername)
+           (ind : mutual_inductive_body) : list (inductive * nat * positive) :=
+  List.concat
+    (mapi
+       (fun i oib =>
+          let ind := {| inductive_mind := kn; inductive_ind := i |} in
+          mapi (fun c '(name, bts) => (ind, c, mask_from_ctor_types bts))
+               (ind_ctors oib))
+       (ind_bodies ind)).
+
+Record used_set := {
+  used_function_params : list (kername * positive);
+  used_ctor_params : list (inductive * nat * positive); }.
+
+Fixpoint find_used_set (Σ : global_env) : used_set :=
+  match Σ with
+  | [] => {| used_ctor_params := []; used_function_params := [] |}
+  | (kn, decl) :: Σ =>
+    let (funcs, ctors) := find_used_set Σ in
+    let (funcs, ctors) :=
+        match decl with
+        | ConstantDecl cst => ((kn, constant_used_params cst) :: funcs, ctors)
+        | InductiveDecl ind => (funcs, ind_ctors_used_params kn ind ++ ctors)
+        end in
+    {| used_function_params := funcs; used_ctor_params := ctors |}
+  end.
+
+Definition remove_unused_args (Σ : global_env) : global_env :=
+  let used_set := find_used_set Σ in
+  let dearg_const_masks := map (on_snd lnot) (used_function_params used_set) in
+  let dearg_ctor_masks := map (fun '(ind, c, use_mask) => (ind, c, lnot use_mask))
+                              (used_ctor_params used_set) in
+  let consts_eta_count := map (on_snd S_last_1) dearg_const_masks in
+  let ctors_eta_count := map (fun '(ind, c, mask) => (ind, c, S_last_1 mask)) dearg_ctor_masks in
+  let Σ := eta_expand_env ctors_eta_count consts_eta_count Σ in
+  dearg_env dearg_ctor_masks dearg_const_masks Σ.
+
+(*
 Local Open Scope nat.
 Fixpoint uses_var (db : nat) (t : term) : bool :=
   match t with
@@ -399,4 +721,4 @@ mark_constants ((kn, decl) :: Σ) := (mark_decl decl, mark_constants Σ)
     };
   mark_decl (InductiveDecl _) := tt.
 
-(* Step 2:
+*)
